\input{../templates/assignment.tex}

\title{	
\normalfont \normalsize 
\textsc{Norwegian University of Science and Technology\\TDT4136 -- Introduction to Artificial Intelligence} \\ [25pt]
\horrule{0.5pt} \\[0.4cm]
\huge Assignment 2:\\ Propositional and Predicate Logics\\
\horrule{2pt} \\[0.5cm]
}

\author{Per Magnus Veierland\\permve@stud.ntnu.no}

\date{\normalsize\today}

\begin{document}

\maketitle

\section{Models and Entailment in Propositional Logic}

\newacro{CNF}{Conjunctive Normal Form}
\newacro{KB}{Knowledge Base}

\begin{enumerate}

\item \textbf{AIMA Exercise 7.1 / 6.1 -- ``Suppose the agent has\ldots''.}

Following is a listing of the inferences, percepts and actions made by the agent. The R-sentences shows the contents of the knowledge base. Relevant new knowledge is underlined when concluded for readability.

\textit{The agent starts in the known safe location [1,1] facing in the right direction.}

\begin{longtable}{rll}
R1: & \underline{$OK_{1,1}$} & Initial knowledge \\
R2: & $OK_{1,1} \Leftrightarrow \neg P_{1,1} \land \neg W_{1,1}$ & Known from game mechanics \\
R3: & \underline{$\neg P_{1,1}$} & From R1 and R2 (Modus P. + and-elimination) \\
R4: & \underline{$\neg W_{1,1}$} & From R1 and R2 (Modus P. + and-elimination) \\
R5: & \underline{$\neg B_{1,1} \land \neg G_{1,1} \land \neg S_{1,1}$} & Percepts in [1,1] \\
R6: & $B_{1,1} \Leftrightarrow P_{1,2} \lor P_{2,1}$ & Known from game mechanics \\
R7: & $(B_{1,1} \Rightarrow P_{1,2} \lor P_{2,1}) \land (P_{1,2} \lor P_{2,1} \Rightarrow B_{1,1})$ & From R6 (Biconditional elimination) \\
R8: & $(P_{1,2} \lor P_{2,1}) \Rightarrow B_{1,1}$ & From R7 (And-elimination) \\
R9: & $\neg B_{1,1} \Rightarrow \neg (P_{1,2} \lor P_{2,1})$ & From R8 (Equivalence of contrapositive) \\
R10: & $\neg (P_{1,2} \lor P_{2,1})$ & From R5 and R9 (Modus Ponens) \\
R11: & \underline{$\neg P_{2,1} \land \neg P_{2,1}$} & From R10 (De Morgan's theorem) \\
R12: & $S_{1,1} \Leftrightarrow W_{1,2} \lor W_{2,1}$ & Known from game mechanics \\
R13: & \underline{$\neg W_{1,2} \land \neg W_{2,1}$} & From R5 and R12 (see R6-R11) \\
R14: & $OK_{1,2} \Leftrightarrow \neg P_{1,2} \land \neg W_{1,2}$ & From game mechanics \\
R15: & $(OK_{1,2} \Rightarrow \neg P_{1,2} \land \neg W_{1,2}) \land (\neg P_{1,2} \land \neg W_{1,2} \Rightarrow OK_{1,2})$ & From R14 (Equivalence of contrapositive) \\
R16: & $\neg P_{1,2} \land \neg W_{1,2} \Rightarrow OK_{1,2}$ & From R15 (And-elimination) \\
R17: & \underline{$OK_{1,2}$} & Modus Ponens to R16 given R11 and R13 \\
R18: & \underline{$OK_{2,1}$} & From R11 and R13 (see R14-R17) \\
\end{longtable}
\addtocounter{table}{-1}

\textit{The agent moves to the known safe location [2,1] facing right. Actions: Forward.}

\begin{longtable}{rll}
R19: & \underline{$B_{2,1} \land \neg G_{2,1} \land \neg S_{2,1}$} & Percepts in [2,1] \\
R20: & $B_{2,1} \Leftrightarrow P_{1,1} \lor P_{2,2} \lor P_{3,1}$ & Known from game mechanics \\
R21: & $P_{1,1} \lor P_{2,2} \lor P_{3,1}$ & From R19 and R20 (Modus Ponens) \\
R22: & \underline{$P_{2,2} \lor P_{3,1}$} & From R3 and R21 (Resolution) \\
R23: & $S_{2,1} \Leftrightarrow W_{1,1} \lor W_{2,2} \lor W_{3,1}$ & Known from game mechanics \\
R24: & $\neg W_{1,1} \land \neg W_{2,2} \land \neg W_{3,1}$ & From R19 and R23 (see R6-R11) \\
R25: & \underline{$\neg W_{2,2} \land \neg W_{3,1}$} & From R4 and R24 (Removed redundancy) \\
\end{longtable}
\addtocounter{table}{-1}

\textit{The agent moves to location [1,2] through location [1,1] as this is the only remaining location known to be safe. Actions: TurnRight, TurnRight, Forward, TurnRight, Forward. The agent faces upwards.}

\begin{longtable}{rll}
R26: & \underline{$\neg B_{1,2} \land \neg G_{1,2} \land S_{1,2}$} & Percepts in [1,2] \\
R27: & $B_{1,2} \Leftrightarrow P_{1,1} \lor P_{2,2} \lor P_{1,3}$ & Known from game mechanics \\
R28: & $\neg P_{1,1} \land \neg P_{1,3} \land \neg P_{2,2}$ & From R26 and R27 (see R6-R11) \\ 
R29: & \underline{$\neg P_{1,3} \land \neg P_{2,2}$} & From R3 and R28 (Removed redundancy) \\
R30: & \underline{$P_{3,1}$} & From R22 and R29 (Resolution) \\
R31: & $OK_{2,2} \Leftrightarrow \neg P_{2,2} \land \neg W_{2,2}$ & Known from game mechanics \\
R32: & \underline{$OK_{2,2}$} & From R25, R29 and R31 (Modus Ponens) \\
R33: & $S_{1,2} \Leftrightarrow W_{1,1} \lor W_{2,2} \lor W_{1,3}$ & Known from game mechanics \\
R34: & $W_{1,1} \lor W_{2,2} \lor W_{1,3}$ & From R26 and R33 (Modus Ponens) \\
R35: & \underline{$W_{1,3}$} & From R4, R25 and R34 (Resolution) \\
R36: & $OK_{1,3} \Leftrightarrow \neg P_{1,3} \land \neg W_{1,3}$ & Known from game mechanics \\
R37: & \underline{$\neg OK_{1,3}$} & From R35 and R36 (see R14-R16) \\
\end{longtable}
\addtocounter{table}{-1}

The knowledge base now contains all percepts and inferences made by the agent after vising locations [1,1], [2,1] and [1,2]. The permutations of possible worlds concerning the locations [1,3], [2,2] and [3,1] together with sentences $\alpha_2 = \neg P_{2,2}$, $\alpha_3 = W_{1,3}$ and the knowledge base ($KB$) is shown in Table~\ref{table:wompus_truths}. 

It is clear that sentences $\alpha_2$ and $\alpha_3$ are true in all models in which $KB$ is true. From this it follows that $KB \vDash \alpha_2$ and that $KB \vDash \alpha_3$.

\newcommand{\F}{{\color{WildStrawberry}\small false}}
\newcommand{\T}{{\color{YellowGreen}\small true}}

\begin{longtable}[c]{c|cccccc|cc|c}
World & $W_{1,3}$ & $W_{2,2}$ & $W_{3,1}$ & $P_{1,3}$ & $P_{2,2}$ & $P_{3,1}$ & $\alpha_2$ & $\alpha_3$ & $KB$ \\ 
\hline
\endhead
1	  & \F        & \F        & \F        & \F        & \F        & \F        & \T         & \F         & \F   \\
2	  & \F        & \F        & \F        & \F        & \F        & \T        & \T         & \F         & \F   \\
3	  & \F        & \F        & \F        & \F        & \T        & \F        & \F         & \F         & \F   \\
4	  & \F        & \F        & \F        & \F        & \T        & \T        & \F         & \F         & \F   \\
5	  & \F        & \F        & \F        & \T        & \F        & \F        & \T         & \F         & \F   \\
6	  & \F        & \F        & \F        & \T        & \F        & \T        & \T         & \F         & \F   \\
7	  & \F        & \F        & \F        & \T        & \T        & \F        & \F         & \F         & \F   \\
8	  & \F        & \F        & \F        & \T        & \T        & \T        & \F         & \F         & \F   \\
9	  & \F        & \F        & \T        & \F        & \F        & \F        & \T         & \F         & \F   \\
10	  & \F        & \F        & \T        & \F        & \F        & \T        & \T         & \F         & \F   \\
11	  & \F        & \F        & \T        & \F        & \T        & \F        & \F         & \F         & \F   \\
12	  & \F        & \F        & \T        & \F        & \T        & \T        & \F         & \F         & \F   \\
13	  & \F        & \F        & \T        & \T        & \F        & \F        & \T         & \F         & \F   \\
14	  & \F        & \F        & \T        & \T        & \F        & \T        & \T         & \F         & \F   \\
15	  & \F        & \F        & \T        & \T        & \T        & \F        & \F         & \F         & \F   \\
16	  & \F        & \F        & \T        & \T        & \T        & \T        & \F         & \F         & \F   \\
17	  & \F        & \T        & \F        & \F        & \F        & \F        & \T         & \F         & \F   \\
18	  & \F        & \T        & \F        & \F        & \F        & \T        & \T         & \F         & \F   \\
19	  & \F        & \T        & \F        & \F        & \T        & \F        & \F         & \F         & \F   \\
20	  & \F        & \T        & \F        & \F        & \T        & \T        & \F         & \F         & \F   \\
21	  & \F        & \T        & \F        & \T        & \F        & \F        & \T         & \F         & \F   \\
22	  & \F        & \T        & \F        & \T        & \F        & \T        & \T         & \F         & \F   \\
23	  & \F        & \T        & \F        & \T        & \T        & \F        & \F         & \F         & \F   \\
24	  & \F        & \T        & \F        & \T        & \T        & \T        & \F         & \F         & \F   \\
25	  & \T        & \F        & \F        & \F        & \F        & \F        & \T         & \T         & \F   \\
26	  & \T        & \F        & \F        & \F        & \F        & \T        & \T         & \T         & \T   \\
27	  & \T        & \F        & \F        & \F        & \T        & \F        & \F         & \T         & \F   \\
28	  & \T        & \F        & \F        & \F        & \T        & \T        & \F         & \T         & \F   \\
29	  & \T        & \F        & \F        & \T        & \F        & \F        & \T         & \T         & \F   \\
30	  & \T        & \F        & \F        & \T        & \F        & \T        & \T         & \T         & \F   \\
31	  & \T        & \F        & \F        & \T        & \T        & \F        & \F         & \T         & \F   \\
32	  & \T        & \F        & \F        & \T        & \T        & \T        & \F         & \T         & \F   \\
\caption{Model table showing $KB$, $\alpha_2$ and $\alpha_3$ truth values (Problem 1.1)}
\label{table:wompus_truths}
\end{longtable}

\item \textbf{AIMA Exercise 7.4 / 6.4 -- ``Which of the following are correct?''.}

\begin{enumerate}
\setcounter{enumii}{2}

\item 
\begin{tabular}{ccc|c|c}
$(A$ & $\land$ & $B)$ & $\vDash$ & $(A \Leftrightarrow B)$\\
\hline
\F & \F & \F & \T & \T \\
\F & \F & \T & \T & \F \\
\T & \F & \F & \T & \F \\
\T & \T & \T & \T & \T \\
\end{tabular}

The sentence $(A \land B) \vDash (A \Leftrightarrow B)$ is true in all models and is therefore valid.

\item
\begin{tabular}{ccc|c|c}
$(A$ & $\Leftrightarrow$ & $B)$ & $\vDash$ & $(A \lor B)$ \\
\hline
\F & \T & \F & \F & \F \\
\F & \F & \T & \T & \T \\
\T & \F & \F & \T & \T \\
\T & \T & \T & \T & \T \\
\end{tabular}

The sentence $(A \Leftrightarrow B) \vDash (A \lor B)$ is not true in all models and is therefore invalid.

\item
\begin{tabular}{ccc|c|ccc}
$(A$ & $\Leftrightarrow$ & $B)$ & $\vDash$ & $(\neg A$ & $\lor$ & $B)$ \\
\hline
\F & \T & \F & \T & \T & \T & \F \\
\F & \F & \T & \T & \T & \T & \T \\
\T & \F & \F & \T & \F & \F & \F \\
\T & \T & \T & \T & \F & \T & \T \\
\end{tabular}

The sentence $(A \Leftrightarrow B) \vDash (\neg A \lor B)$ is true in all models and is therefore valid.

\item
\begin{tabular}{ccccc|c|ccc}
$(A$ & $\land$ & $B)$ & $\Rightarrow$ & $C$ & $\vDash$ & $(A \Rightarrow C)$ & $\lor$ & $(B \Rightarrow C)$\\
\hline
\F & \F & \F & \T & \F & \T & \T & \T & \T\\
\F & \F & \F & \T & \T & \T & \T & \T & \T\\
\F & \F & \T & \T & \F & \T & \T & \T & \F\\
\F & \F & \T & \T & \T & \T & \T & \T & \T\\
\T & \F & \F & \T & \F & \T & \F & \T & \T\\
\T & \F & \F & \T & \T & \T & \T & \T & \T\\
\T & \T & \T & \F & \F & \T & \F & \F & \F\\
\T & \T & \T & \T & \T & \T & \T & \T & \T\\
\end{tabular}

The sentence $\big((A \land B) \Rightarrow C\big) \vDash \big((A \Rightarrow C) \lor (B \Rightarrow C)\big)$ is true in all models and is therefore valid.

\item
\begin{tabular}{ccccc|c|ccccccc}
$C$ & $\lor$ & $(\neg A$ & $\land$ & $\neg B)$ & $\equiv$ & $(A$ & $\Rightarrow$ & $C)$ & $\land$ & $(B$ & $\Rightarrow$ & $C)$\\
\hline
\F & \T & \T & \T & \T & \T & \F & \T & \F & \T & \F & \T & \F \\
\T & \T & \T & \T & \T & \T & \F & \T & \T & \T & \F & \T & \T \\
\F & \F & \T & \F & \F & \T & \F & \T & \F & \F & \T & \F & \F \\
\T & \T & \T & \F & \F & \T & \F & \T & \T & \T & \T & \T & \T \\
\F & \F & \F & \F & \T & \T & \T & \F & \F & \F & \F & \T & \F \\
\T & \T & \F & \F & \T & \T & \T & \T & \T & \T & \F & \T & \T \\
\F & \F & \F & \F & \F & \T & \T & \F & \F & \F & \T & \F & \F \\
\T & \T & \F & \F & \F & \T & \T & \T & \T & \T & \T & \T & \T \\
\end{tabular}

The sentence $C \lor (\neg A \land \neg B) \equiv (A \Rightarrow C) \land (B \Rightarrow C)$ is true in all models and is therefore valid.

\item
\begin{tabular}{ccccccccc|c|c}
$(A$ & $\lor$ & $B)$ & $\land$ & $\big(\neg C$ & $\lor$ & $(\neg D$ & $\lor$ & $E)\big)$ & $\vDash$ & $(A \lor B)$\\
\hline
\F & \F & \F & \F & \T & \T & \T & \T & \F & \T & \F \\
\F & \F & \F & \F & \T & \T & \T & \T & \T & \T & \F \\
\F & \F & \F & \F & \T & \T & \F & \F & \F & \T & \F \\
\F & \F & \F & \F & \T & \T & \F & \T & \T & \T & \F \\
\F & \F & \F & \F & \F & \T & \T & \T & \F & \T & \F \\
\F & \F & \F & \F & \F & \T & \T & \T & \T & \T & \F \\
\F & \F & \F & \F & \F & \F & \F & \F & \F & \T & \F \\
\F & \F & \F & \F & \F & \T & \F & \T & \T & \T & \F \\
\F & \T & \T & \T & \T & \T & \T & \T & \F & \T & \T \\
\F & \T & \T & \T & \T & \T & \T & \T & \T & \T & \T \\
\F & \T & \T & \T & \T & \T & \F & \F & \F & \T & \T \\
\F & \T & \T & \T & \T & \T & \F & \T & \T & \T & \T \\
\F & \T & \T & \T & \F & \T & \T & \T & \F & \T & \T \\
\F & \T & \T & \T & \F & \T & \T & \T & \T & \T & \T \\
\F & \T & \T & \F & \F & \F & \F & \F & \F & \T & \T \\
\F & \T & \T & \T & \F & \T & \F & \T & \T & \T & \T \\
\T & \T & \F & \T & \T & \T & \T & \T & \F & \T & \T \\
\T & \T & \F & \T & \T & \T & \T & \T & \T & \T & \T \\
\T & \T & \F & \T & \T & \T & \F & \F & \F & \T & \T \\
\T & \T & \F & \T & \T & \T & \F & \T & \T & \T & \T \\
\T & \T & \F & \T & \F & \T & \T & \T & \F & \T & \T \\
\T & \T & \F & \T & \F & \T & \T & \T & \T & \T & \T \\
\T & \T & \F & \F & \F & \F & \F & \F & \F & \T & \T \\
\T & \T & \F & \T & \F & \T & \F & \T & \T & \T & \T \\
\T & \T & \T & \T & \T & \T & \T & \T & \F & \T & \T \\
\T & \T & \T & \T & \T & \T & \T & \T & \T & \T & \T \\
\T & \T & \T & \T & \T & \T & \F & \F & \F & \T & \T \\
\T & \T & \T & \T & \T & \T & \F & \T & \T & \T & \T \\
\T & \T & \T & \T & \F & \T & \T & \T & \F & \T & \T \\
\T & \T & \T & \T & \F & \T & \T & \T & \T & \T & \T \\
\T & \T & \T & \F & \F & \F & \F & \F & \F & \T & \T \\
\T & \T & \T & \T & \F & \T & \F & \T & \T & \T & \T \\
\end{tabular}

The sentence $(A \lor B) \land (\neg C \lor \neg D \lor E) \vDash (A \lor B)$ is true in all models and is therefore valid. In the model table the sentence $(\neg C \lor \neg D \lor E)$ has been rewritten as $\neg C \lor (\neg D \lor E)$ to ease formatting (by the associativity of $\lor$).

\item
\begin{tabular}{ccccccccc|c|ccc}
$(A$ & $\lor$ & $B)$ & $\land$ & $\big(\neg C$ & $\lor$ & $(\neg D$ & $\lor$ & $E)\big)$ & $\vDash$ & $(A \lor B)$ & $\land$ & $(\neg D \lor E)$\\
\hline
\F & \F & \F & \F & \T & \T & \T & \T & \F & \T & \F& \F & \T \\
\F & \F & \F & \F & \T & \T & \T & \T & \T & \T & \F& \F & \T \\
\F & \F & \F & \F & \T & \T & \F & \F & \F & \T & \F& \F & \F \\
\F & \F & \F & \F & \T & \T & \F & \T & \T & \T & \F& \F & \T \\
\F & \F & \F & \F & \F & \T & \T & \T & \F & \T & \F& \F & \T \\
\F & \F & \F & \F & \F & \T & \T & \T & \T & \T & \F& \F & \T \\
\F & \F & \F & \F & \F & \F & \F & \F & \F & \T & \F& \F & \F \\
\F & \F & \F & \F & \F & \T & \F & \T & \T & \T & \F& \F & \T \\
\F & \T & \T & \T & \T & \T & \T & \T & \F & \T & \T& \T & \T \\
\F & \T & \T & \T & \T & \T & \T & \T & \T & \T & \T& \T & \T \\
\F & \T & \T & \T & \T & \T & \F & \F & \F & \F & \T& \F & \F \\
\F & \T & \T & \T & \T & \T & \F & \T & \T & \T & \T& \T & \T \\
\F & \T & \T & \T & \F & \T & \T & \T & \F & \T & \T& \T & \T \\
\F & \T & \T & \T & \F & \T & \T & \T & \T & \T & \T& \T & \T \\
\F & \T & \T & \F & \F & \F & \F & \F & \F & \T & \T& \F & \F \\
\F & \T & \T & \T & \F & \T & \F & \T & \T & \T & \T& \T & \T \\
\T & \T & \F & \T & \T & \T & \T & \T & \F & \T & \T& \T & \T \\
\T & \T & \F & \T & \T & \T & \T & \T & \T & \T & \T& \T & \T \\
\T & \T & \F & \T & \T & \T & \F & \F & \F & \F & \T& \F & \F \\
\T & \T & \F & \T & \T & \T & \F & \T & \T & \T & \T& \T & \T \\
\T & \T & \F & \T & \F & \T & \T & \T & \F & \T & \T& \T & \T \\
\T & \T & \F & \T & \F & \T & \T & \T & \T & \T & \T& \T & \T \\
\T & \T & \F & \F & \F & \F & \F & \F & \F & \T & \T& \F & \F \\
\T & \T & \F & \T & \F & \T & \F & \T & \T & \T & \T& \T & \T \\
\T & \T & \T & \T & \T & \T & \T & \T & \F & \T & \T& \T & \T \\
\T & \T & \T & \T & \T & \T & \T & \T & \T & \T & \T& \T & \T \\
\T & \T & \T & \T & \T & \T & \F & \F & \F & \F & \T& \F & \F \\
\T & \T & \T & \T & \T & \T & \F & \T & \T & \T & \T& \T & \T \\
\T & \T & \T & \T & \F & \T & \T & \T & \F & \T & \T& \T & \T \\
\T & \T & \T & \T & \F & \T & \T & \T & \T & \T & \T& \T & \T \\
\T & \T & \T & \F & \F & \F & \F & \F & \F & \T & \T& \F & \F \\
\T & \T & \T & \T & \F & \T & \F & \T & \T & \T & \T& \T & \T \\
\end{tabular}

The sentence $(A \lor B) \land (\neg C \lor \neg D \lor E) \vDash (A \lor B) \land (\neg D \lor E)$ is not true in all models and is therefore not valid. In the model table the sentence $(\neg C \lor \neg D \lor E)$ has been rewritten as $\neg C \lor (\neg D \lor E)$ to ease formatting (by the associativity of $\lor$).

\item
\begin{tabular}{ccc|c|cc}
$(A$ & $\lor$ & $B)$ & $\land$ & $\neg$ & $(A \Rightarrow B)$\\
\hline
\F & \F & \F & \F & \F & \T \\
\F & \T & \T & \F & \F & \T \\
\T & \T & \F & \T & \T & \F \\
\T & \T & \T & \F & \F & \T \\
\end{tabular}

The model $A \land \neg B$ satisfies the sentence $(A \lor B) \land \neg (A \Rightarrow B)$.

\item
\begin{tabular}{ccc|c|ccc}
$(A$ & $\Leftrightarrow$ & $B)$ & $\land$ & $(\neg A$ & $\lor$ & $B)$\\
\hline
\F & \T & \F & \T & \T & \T & \F \\
\F & \F & \T & \F & \T & \T & \T \\
\T & \F & \F & \F & \F & \F & \F \\
\T & \T & \T & \T & \F & \T & \T \\
\end{tabular}

The models $\neg A \land \neg B$ and $A \land B$ both satisfy the sentence $(A \Leftrightarrow B) \land (\neg A \lor B)$.

\item
\begin{tabular}{ccc|c|c}
$(A$ & $\Leftrightarrow$ & $B)$ & $\Leftrightarrow$ & $C$\\
\hline
\F & \T & \F & \F & \F\\
\F & \T & \F & \T & \T\\
\F & \F & \T & \T & \F\\
\F & \F & \T & \F & \T\\
\T & \F & \F & \T & \F\\
\T & \F & \F & \F & \T\\
\T & \T & \T & \F & \F\\
\T & \T & \T & \T & \T\\
\end{tabular}

The sentence $(A \Leftrightarrow B)$ is satisfied by four models, which is the same number of models which satisfies $(A \Leftrightarrow B) \Leftrightarrow C$.

\end{enumerate}

\item \textbf{Consider a logical knowledge base with 100 variables, $A_1$, $A_2$, \ldots, $A_{100}$. This will have $Q = 2^{100}$ possible models. For each logical sentence below, give the number of models that satisfy it.}

\begin{enumerate}

\item
$\big(\frac{1}{2} \cdot \frac{1}{2}\big) \cdot 2^{100} =
\frac{1}{4} \cdot 2^{100} =
\frac{2^{100}}{2^2} =
2^{98}$

The logical sentence $A_{24} \land A_{50}$ is satisfied by $2^{98}$ models.

\item
$\big(\frac{1}{2} + \frac{1}{2} - \frac{1}{2} \cdot \frac{1}{2}\big) \cdot 2^{100} =
\big(1 - \frac{1}{4}\big) \cdot 2^{100} =
\frac{3}{4} \cdot 2^{100} =
\frac{3 \cdot 2^{100}}{2^2} =
3 \cdot 2^{98}$

The logical sentence $\neg A_{38} \lor \neg A_{47}$ is satisfied by $3 \cdot 2^{98}$ models.

\item
To simplify the calculation the logical sentence $(A_{1} \lor \neg A_{57}) \land (A_{1} \lor \neg A_{99})$ can be rewritten as $(A_{1} \lor (\neg A_{57} \land \neg A_{99}))$ by the distributivity of $\lor$ over $\land$.

$\big(\frac{1}{2} + \frac{1}{2} \cdot \frac{1}{2} - \frac{1}{2} \cdot \frac{1}{2} \cdot \frac{1}{2}\big) \cdot 2^{100} =
\big(\frac{4}{8} + \frac{2}{8} - \frac{1}{8}\big) \cdot 2^{100} =
\frac{5}{8} \cdot 2^{100} =
\frac{5 \cdot 2^{100}}{2^3} =
5 \cdot 2^{97}$

The logical sentence $(A_{1} \lor \neg A_{57}) \land (A_{1} \lor \neg A_{99})$ is satisfied by $5 \cdot 2^{97}$ models.

\item
$\big(\frac{1}{2} \cdot \frac{1}{2} + \frac{1}{2} \cdot \frac{1}{2}\big) \cdot 2^{100} =
\big(\frac{1}{4} + \frac{1}{4}\big) \cdot 2^{100} =
\frac{1}{2} \cdot 2^{100} =
\frac{2^{100}}{2^1} =
2^{99}$

The logical sentence $A_{58} \Leftrightarrow A_{90}$ is satisfied by $2^{99}$ models.

\item
$\big(\frac{1}{2}\big)^{6} \cdot 2^{100} =
\frac{2^{100}}{2^6} =
2^{94}$

The logical sentence $A_1 \land \neg A_2 \land A_3 \land \neg A_4 \land A_5 \land \neg A_6$ is satisfied by $2^{94}$ models.

\item
$\Big(\big(\frac{1}{2}\big)^{50} + \big(\frac{1}{2}\big)^{50} - \big(\frac{1}{2}\big)^{50} \cdot \big(\frac{1}{2}\big)^{50}\Big) \cdot 2^{100} =
\Big(2 \cdot \big(\frac{1}{2}\big)^{50} - \big(\frac{1}{2}\big)^{100}\Big) \cdot 2^{100} = \\
\Big(\frac{2}{2^{50}} - \frac{1}{2^{100}}\Big) \cdot 2^{100} =
\frac{2^{100}}{2^{49}} - \frac{2^{100}}{2^{100}} =
2^{51} - 1$

The logical sentence $(\neg A_1 \land \neg A_2 \land \ldots \land \neg A_{50}) \lor (A_{51} \land A_{52} \land \ldots \land A_{100})$ is satisfied by $2^{51} - 1$ models.

\item
$\Big(\big(\frac{1}{2}\big)^3 + \big(\frac{1}{2}\big)^3 - \big(\frac{1}{2}\big)^3 \cdot \big(\frac{1}{2}\big)^3\Big) \cdot 2^{100} =
\big(\frac{2}{8} - \frac{1}{64}\big) \cdot 2^{100} =
\frac{15}{64} \cdot 2^{100} =
\frac{15 \cdot 2^{100}}{2^6} =
15 \cdot 2^{94}$

The logical sentence $(A_1 \land A_2 \land A_3) \lor (A_4 \land A_5 \land A_6)$ is satisfied by $15 \cdot 2^{94}$ models.

\end{enumerate}

\end{enumerate}

\section{Resolution in Propositional Logic}

\begin{enumerate}

\item \textbf{Convert each of the following sentences to \acf{CNF}.}

\begin{enumerate}

\item $A \land \neg B \land C \equiv \underline{(A) \land (\neg B) \land (C)}$

\item $\neg A \lor \neg B \lor \neg C \equiv \underline{(\neg A \lor \neg B \lor \neg C)}$

\item
$(\neg A \land B) \Rightarrow C \equiv
\neg (\neg A \land B) \lor C \equiv
\neg \neg A \lor \neg B \lor C \equiv
\underline{(A \lor \neg B \lor C)}$

\item
$(A \lor B) \Rightarrow \neg C \equiv
\neg (A \lor B) \lor \neg C \equiv
(\neg A \land \neg B) \lor \neg C \equiv
\underline{(\neg A \lor \neg C) \land (\neg B \lor \neg C)}$

\item
$(A \land B) \Leftrightarrow (C \land D) \equiv$\\
$(A \land B \Rightarrow C \land D) \land (C \land D \Rightarrow A \land B) \equiv$\\
$\big(\neg (A \land B) \lor (C \land D)\big) \land \big(\neg (C \land D) \lor (A \land B)\big) \equiv$\\
$\big(\neg (A \land B) \land \neg (C \land D)\big) \lor \big(\neg (A \land B) \land (A \land B)\big) \lor \big((C \land D) \land \neg (C \land D)\big) \lor \big((C \land D) \land (A \land B)\big) \equiv$\\
$\big(\neg (A \land B) \land \neg (C \land D)\big) \lor \big((C \land D) \land (A \land B)\big) \equiv$\\
$\big((\neg A \lor \neg B) \land (\neg C \lor \neg D)\big) \lor (A \land B \land C \land D) \equiv$\\
$\big((\neg A \lor \neg B) \lor (A \land B \land C \land D)\big) \land \big((\neg C \lor \neg D) \lor (A \land B \land C \land D)\big) \equiv $ 

$(\neg A \lor \neg B \lor A) \land (\neg A \lor \neg B \lor B) \land (\neg A \lor \neg B \lor C) \land (\neg A \lor \neg B \lor D) \land\\(\neg C \lor \neg D \lor A) \land (\neg C \lor \neg D \lor B) \land (\neg C \lor \neg D \lor C) \land (\neg C \lor \neg D \lor D) \equiv $ 

\underline{$(A \lor \neg C \lor \neg D) \land (\neg A \lor \neg B \lor C) \land (\neg A \lor \neg B \lor D) \land (B \lor \neg C \lor \neg D)$}

\end{enumerate}

\item \textbf{Consider the following \acf{KB}:}

\begin{itemize}
\item $(B \lor \neg C) \Rightarrow \neg A$
\item $(\neg A \lor D) \Rightarrow B$
\item $A \land C$
\end{itemize}

\textbf{Use resolution to show that $KB \vDash \neg D$.}

To use resolution we begin with converting the knowledge base to \ac{CNF} since the resolution rule only applies to disjunctions of literals.

\begin{itemize}
\item $(B \lor \neg C) \Rightarrow \neg A \equiv \neg (B \lor \neg C) \lor \neg A \equiv (\neg B \land C) \lor \neg A \equiv \underline{(\neg B \lor \neg A) \land (C \lor \neg A)}$
\item $(\neg A \lor D) \Rightarrow B \equiv \neg (\neg A \lor D) \lor B \equiv (A \land \neg D) \lor B \equiv \underline{(A \lor B) \land (B \lor \neg D)}$
\item $A \land C \equiv \underline{(A) \land (C)}$
\end{itemize}

Proving entailment by resolution is done by showing a contradiction. To prove that $KB \vDash \neg D$ we show that $KB \land D$ is unsatisfiable.

$KB \land D = (\neg B \lor \neg A) \land (C \lor \neg A) \land (A \lor B) \land (B \lor \neg D) \land (A) \land (C) \land (D)$

\begin{enumerate}
\item $\frac{(\neg B \lor \neg A),\quad (B \lor \neg D)}{\neg A \lor \neg D}$
\item $\frac{(\neg A \lor \neg D),\quad (D)}{\neg A}$
\item $\frac{\neg A,\quad A}{\textit{False}}$
\end{enumerate}

Since \textit{False} can be inferred from two clauses which must be true it is clear that there is a contradiction in the set of clauses. This contradiction proves that $KB \vDash D$ is unsatisfiable and therefore that $KB \vDash \neg D$ must be true.

\end{enumerate}

\end{document}

